theories/logrel/F_mu_ref_conc/wp_rules.v
@@ -140,7 +140,8 @@ Section lang_rules.
     iNext; iIntros (v2 σ2 efs Hstep) "_"; inv_base_step. by iFrame.
   Qed.
 
-  Local Ltac solve_exec_safe := intros; subst; do 3 eexists; econstructor; eauto.
+  Local Ltac solve_exec_safe :=
+    intros; subst; do 3 eexists; econstructor; simpl; eauto.
   Local Ltac solve_exec_puredet := simpl; intros; by inv_base_step.
   Local Ltac solve_pure_exec :=
     unfold IntoVal in *;
@@ -199,8 +200,33 @@ Section lang_rules.
     PureExec True 1 (If (#♭ false) e1 e2) e2.
   Proof. solve_pure_exec. Qed.
 
-  Global Instance wp_nat_binop op a b :
-    PureExec True 1 (BinOp op (#n a) (#n b)) (of_val (binop_eval op a b)).
-  Proof. solve_pure_exec. Qed.
+  Global Instance wp_int_binop op a b :
+    PureExec True 1 (BinOp op (#n a) (#n b)) (of_val (int_binop_eval op a b)).
+  Proof.
+    destruct op;
+      (unfold IntoVal in *;
+      repeat match goal with H : AsVal _ |- _ => destruct H as [??] end; subst;
+       intros ?; apply nsteps_once, pure_base_step_pure_step;
+       constructor; [solve_exec_safe |try solve_exec_puredet]); [].
+    intros; simpl in *; inv_base_step.
+    destruct Z.eq_dec as [->|];
+      [rewrite bool_decide_eq_true_2; done|
+       rewrite bool_decide_eq_false_2; eauto with congruence].
+  Qed.
+
+  Global Instance wp_Eq_binop `{!AsVal e1} `{!AsVal e2} :
+    PureExec True 1 (BinOp Eq e1 e2) (#♭ (bool_decide (e1 = e2))).
+  Proof.
+    unfold IntoVal in *;
+      repeat match goal with H : AsVal _ |- _ => destruct H as [??] end; subst;
+       intros ?; apply nsteps_once, pure_base_step_pure_step;
+       constructor; [solve_exec_safe |]; [].
+    intros; simpl in *; inv_base_step.
+    match goal with |- context[ bool_decide (?A = ?B)] =>
+    destruct (decide (A = B)) as [->|] end;
+    [rewrite !bool_decide_eq_true_2; done|
+       rewrite !bool_decide_eq_false_2; eauto].
+    intros ?%of_val_inj; done.
+  Qed.
 
 End lang_rules.
